SaberPKE/SaberPKESecurity.ec
@@ -15,7 +15,7 @@ require import SaberPKEPreliminaries.
 (*---*) import DMapRqv2Rpv.
 
 (* ----------------------------------- *)
-(*  Adversary Prototypes               *)
+(*  Adversary Classes                  *)
 (* ----------------------------------- *)
 
 module type Adv_GMLWR = {
@@ -25,6 +25,22 @@ module type Adv_GMLWR = {
 module type Adv_XMLWR = {
    proc guess(sd : seed, b : Rp_vec, a : Rq_vec, d : Rp) : bool
 }.
+
+module type Adv_INDCPA = {
+  proc choose(pk : seed * Rp_vec) : R2 * R2  
+  proc guess(c : R2t * Rp_vec) : bool
+}.
+
+module type Adv_INDCPA_2 = {
+  proc choose(pk : seed * Rp_vec) : R2 * R2  
+  proc guess(c : Rppq * Rp_vec) : bool
+}.
+
+module type Adv_INDCPA_34 = {
+  proc choose(pk : seed * Rq_vec) : R2 * R2  
+  proc guess(c : Rp * Rp_vec) : bool
+}.
+
 
 (* ----------------------------------- *)
 (*  Games                              *)
@@ -93,10 +109,10 @@ module XMLWR(A : Adv_XMLWR) = {
 
 (* --- Game Sequence --- *)
 (* Game 0 *)
-module Game0(A : Adversary) = {
+module Game0(A : Adv_INDCPA) = {
    proc main() : bool = {
       var u, u' : bool;
-      var m0, m1 : plaintext;
+      var m0, m1 : R2;
 
       var sd : seed;
       var _A : Rq_mat;
@@ -112,24 +128,24 @@ module Game0(A : Adversary) = {
       s <$ dsmallRq_vec;
       b <- scaleRqv2Rpv (_A *^ s + h);
 
-      (m0, m1) <@ A.choose(pk_encode_g (sd, b));
+      (m0, m1) <@ A.choose((sd, b));
 
       s' <$ dsmallRq_vec;
       b' <- scaleRqv2Rpv ((trmx _A) *^ s' + h);
       v' <- (dotp b (Rqv2Rpv s')) + (Rq2Rp h1);
-      cmu <- scaleRp2R2t (v' + (scaleR22Rp (m_decode (if u then m1 else m0))));
+      cmu <- scaleRp2R2t (v' + (scaleR22Rp (if u then m1 else m0)));
       
-      u' <@ A.guess(c_encode_g (cmu, b'));
+      u' <@ A.guess((cmu, b'));
 
       return (u = u');
    }
 }.
 
 (* Game 1 *)
-module Game1(A : Adversary) = {
+module Game1(A : Adv_INDCPA) = {
    proc main() : bool = {
       var u, u' : bool;
-      var m0, m1 : plaintext;
+      var m0, m1 : R2;
 
       var sd : seed;
       var _A : Rq_mat;
@@ -145,24 +161,24 @@ module Game1(A : Adversary) = {
       (* Skip: s <$ dsmallRq_vec; *)
       b <$ dRp_vec;
 
-      (m0, m1) <@ A.choose(pk_encode_g (sd, b));
+      (m0, m1) <@ A.choose((sd, b));
 
       s' <$ dsmallRq_vec;
       b' <- scaleRqv2Rpv ((trmx _A) *^ s' + h);
       v' <- (dotp b (Rqv2Rpv s')) + (Rq2Rp h1);
-      cmu <- scaleRp2R2t (v' + (scaleR22Rp (m_decode (if u then m1 else m0))));
+      cmu <- scaleRp2R2t (v' + (scaleR22Rp (if u then m1 else m0)));
       
-      u' <@ A.guess(c_encode_g (cmu, b'));
+      u' <@ A.guess((cmu, b'));
 
       return (u = u');
    }
 }.
 
 (* Game 2 *)
-module Game2(A : Adversary) = {
+module Game2(A : Adv_INDCPA_2) = {
    proc main() : bool = {
       var u, u' : bool;
-      var m0, m1 : plaintext;
+      var m0, m1 : R2;
 
       var sd : seed;
       var _A : Rq_mat;
@@ -178,24 +194,24 @@ module Game2(A : Adversary) = {
       (* Skip: s <$ dsmallRq_vec; *)
       b <$ dRp_vec;
 
-      (m0, m1) <@ A.choose(pk_encode_g (sd, b));
+      (m0, m1) <@ A.choose((sd, b));
 
       s' <$ dsmallRq_vec;
       b' <- scaleRqv2Rpv ((trmx _A) *^ s' + h);
       v' <- (dotp b (Rqv2Rpv s')) + (Rq2Rp h1);
-      cmu <- scaleRp2Rppq (v' + (scaleR22Rp (m_decode (if u then m1 else m0))));
+      cmu <- scaleRp2Rppq (v' + (scaleR22Rp (if u then m1 else m0)));
       
-      u' <@ A.guess(c_encode_g (cmu, b'));
+      u' <@ A.guess((cmu, b'));
 
       return (u = u');
    }
 }.
 
 (* Auxiliary Game (Reduction 2-3): Game 2a *)
-module Game2a(A : Adversary) = {
+module Game2a(A : Adv_INDCPA_2) = {
    proc main() : bool = {
       var u, u' : bool;
-      var m0, m1 : plaintext;
+      var m0, m1 : R2;
 
       var sd : seed;
       var _A : Rq_mat;
@@ -211,24 +227,24 @@ module Game2a(A : Adversary) = {
       (* Skip: s <$ dsmallRq_vec; *)
       b <@ Rqv2RpvSampl.sample(dRq_vec, Rqv2Rpv);
 
-      (m0, m1) <@ A.choose(pk_encode_g (sd, b));
+      (m0, m1) <@ A.choose((sd, b));
 
       s' <$ dsmallRq_vec;
       b' <- scaleRqv2Rpv ((trmx _A) *^ s' + h);
       v' <- (dotp b (Rqv2Rpv s')) + (Rq2Rp h1);
-      cmu <- scaleRp2Rppq (v' + (scaleR22Rp (m_decode (if u then m1 else m0))));
+      cmu <- scaleRp2Rppq (v' + (scaleR22Rp (if u then m1 else m0)));
       
-      u' <@ A.guess(c_encode_g (cmu, b'));
+      u' <@ A.guess((cmu, b'));
 
       return (u = u');
    }
 }.
 
 (* Auxiliary Game (Reduction 2-3): Game 2b *)
-module Game2b(A : Adversary) = {
+module Game2b(A : Adv_INDCPA_2) = {
    proc main() : bool = {
       var u, u' : bool;
-      var m0, m1 : plaintext;
+      var m0, m1 : R2;
 
       var sd : seed;
       var _A : Rq_mat;
@@ -245,24 +261,24 @@ module Game2b(A : Adversary) = {
       (* Skip: s <$ dsmallRq_vec; *)
       b <@ Rqv2RpvSampl.map(dRq_vec, Rqv2Rpv);
 
-      (m0, m1) <@ A.choose(pk_encode_g (sd, b));
+      (m0, m1) <@ A.choose((sd, b));
 
       s' <$ dsmallRq_vec;
       b' <- scaleRqv2Rpv ((trmx _A) *^ s' + h);
       v' <- (dotp b (Rqv2Rpv s')) + (Rq2Rp h1);
-      cmu <- scaleRp2Rppq (v' + (scaleR22Rp (m_decode (if u then m1 else m0))));
+      cmu <- scaleRp2Rppq (v' + (scaleR22Rp (if u then m1 else m0)));
       
-      u' <@ A.guess(c_encode_g (cmu, b'));
+      u' <@ A.guess((cmu, b'));
 
       return (u = u');
    }
 }.
 
 (* Game 3 *)
-module Game3(A : Adversary) = {
+module Game3(A : Adv_INDCPA_34) = {
    proc main() : bool = {
       var u, u' : bool;
-      var m0, m1 : plaintext;
+      var m0, m1 : R2;
 
       var sd : seed;
       var _A : Rq_mat;
@@ -279,24 +295,24 @@ module Game3(A : Adversary) = {
       (* Skip: s <$ dsmallRq_vec; *)
       b <$ dRq_vec;
 
-      (m0, m1) <@ A.choose(pk_encode_g (sd, b));
+      (m0, m1) <@ A.choose((sd, b));
 
       s' <$ dsmallRq_vec;
       b' <- scaleRqv2Rpv ((trmx _A) *^ s' + h);
       v' <- scaleRq2Rp ((dotp b s') + h1);
-      cmu <- v' + (scaleR22Rp_var (m_decode (if u then m1 else m0)) (2 * ep - eq - 1));
+      cmu <- v' + (scaleR22Rp_var (if u then m1 else m0) (2 * ep - eq - 1));
    
-      u' <@ A.guess(c_encode_g (cmu, b'));
+      u' <@ A.guess((cmu, b'));
 
       return (u = u');
    }
 }.
 
 (* Game 4 *)
-module Game4(A : Adversary) = {
+module Game4(A : Adv_INDCPA_34) = {
    proc main() : bool = {
       var u, u' : bool;
-      var m0, m1 : plaintext;
+      var m0, m1 : R2;
 
       var sd : seed;
       var _A : Rq_mat;
@@ -313,24 +329,24 @@ module Game4(A : Adversary) = {
       (* Skip: s <$ dsmallRq_vec; *)
       b <$ dRq_vec;
 
-      (m0, m1) <@ A.choose(pk_encode_g (sd, b));
+      (m0, m1) <@ A.choose((sd, b));
 
       (* Skip: s' <$ dsmallRq_vec; *)
       b' <$ dRp_vec;
       v' <$ dRp;
-      cmu <- v' + (scaleR22Rp_var (m_decode (if u then m1 else m0)) (2 * ep - eq - 1));
+      cmu <- v' + (scaleR22Rp_var (if u then m1 else m0) (2 * ep - eq - 1));
       
-      u' <@ A.guess(c_encode_g (cmu, b'));
+      u' <@ A.guess((cmu, b'));
 
       return (u = u');
    }
 }.
 
 (* Auxiliary Game with All Random Artifacts *)
-module Auxiliary_Game(A : Adversary) = {
+module Auxiliary_Game(A : Adv_INDCPA_34) = {
    proc main() : bool = {
       var u, u' : bool;
-      var m0, m1 : plaintext;
+      var m0, m1 : R2;
       
       var sd : seed;
       var b : Rq_vec;
@@ -340,12 +356,12 @@ module Auxiliary_Game(A : Adversary) = {
       sd <$ dseed;
       b <$ dRq_vec;
       
-      (m0, m1) <@ A.choose(pk_encode_g (sd, b));
+      (m0, m1) <@ A.choose((sd, b));
        
       b' <$ dRp_vec;
       cmu <$ dRp;
          
-      u' <@ A.guess(c_encode_g (cmu, b'));
+      u' <@ A.guess((cmu, b'));
       
       u <$ dbool;
 
@@ -359,10 +375,10 @@ module Auxiliary_Game(A : Adversary) = {
 
 (* --- MLWR-Related Adversaries --- *)
 (* Adversary B0 Against GMLWR, Constructed from Adversary A Distinguishing Between Game0 and Game1 *)
-module B0(A : Adversary) : Adv_GMLWR = {
+module B0(A : Adv_INDCPA) : Adv_GMLWR = {
    proc guess(sd : seed, b : Rp_vec) : bool = {
       var w, w' : bool;
-      var m0, m1 : plaintext;
+      var m0, m1 : R2;
       
       var _A : Rq_mat;
       var s' : Rq_vec;
@@ -374,34 +390,34 @@ module B0(A : Adversary) : Adv_GMLWR = {
 
       _A <- gen sd;
 
-      (m0, m1) <@ A.choose(pk_encode_g (sd, b));
+      (m0, m1) <@ A.choose((sd, b));
 
       s' <$ dsmallRq_vec;
       b' <- scaleRqv2Rpv ((trmx _A) *^ s' + h);
       v' <- (dotp b (Rqv2Rpv s')) + (Rq2Rp h1);
-      cmw <- scaleRp2R2t (v' + (scaleR22Rp (m_decode (if w then m1 else m0))));
+      cmw <- scaleRp2R2t (v' + (scaleR22Rp (if w then m1 else m0)));
       
-      w' <@ A.guess(c_encode_g (cmw, b'));
+      w' <@ A.guess((cmw, b'));
       
       return (w = w');
    }
 }.
 
 (* Adversary B1 Against XMLWR, Constructed from Adversary A Distinguishing between Game3 and Game4 *)
-module B1(A : Adversary) : Adv_XMLWR = {
+module B1(A : Adv_INDCPA_34) : Adv_XMLWR = {
    proc guess(sd : seed, b : Rp_vec, a : Rq_vec, d : Rp) : bool =  {
       var w, w' : bool;
-      var m0, m1 : plaintext;
+      var m0, m1 : R2;
       
       var cmw : Rp;
       
       w <$ dbool;
 
-      (m0, m1) <@ A.choose(pk_encode_g (sd, a));
+      (m0, m1) <@ A.choose((sd, a));
 
-      cmw <- d + (scaleR22Rp_var (m_decode (if w then m1 else m0)) (2 * ep - eq - 1));
+      cmw <- d + (scaleR22Rp_var (if w then m1 else m0) (2 * ep - eq - 1));
       
-      w' <@ A.guess(c_encode_g (cmw, b));
+      w' <@ A.guess((cmw, b));
       
       return (w = w');
    }
@@ -409,69 +425,63 @@ module B1(A : Adversary) : Adv_XMLWR = {
 
 (* --- Other Adversaries --- *)
 (* Adversary A2 Against Game2, Constructed from Adversary A1 Against Game1 *)
-module A2(A1 : Adversary) : Adversary = {
-   proc choose(pk : pkey) : plaintext * plaintext = {
-      var m0, m1 : plaintext;
+module A2(A1 : Adv_INDCPA) : Adv_INDCPA_2 = {
+   proc choose(pk : seed * Rp_vec) : R2 * R2 = {
+      var m0, m1 : R2;
       
       (m0, m1) <@ A1.choose(pk);
       
       return (m0, m1);
    }
 
-   proc guess(c : ciphertext) : bool = {
+   proc guess(c : Rppq * Rp_vec) : bool = {
       var u' : bool;
-      var c_dec : Rppq * Rp_vec;
-
+      
       var cmu : Rppq;
       var b' : Rp_vec;
       var cmu' : R2t;
       
-      c_dec <- c_decode_g c;
-      cmu <- c_dec.`1;
-      b' <- c_dec.`2;
+      cmu <- c.`1;
+      b' <- c.`2;
 
       cmu' <- scaleRppq2R2t cmu; 
             
-      u' <@ A1.guess(c_encode_g (cmu', b'));
+      u' <@ A1.guess((cmu', b'));
 
       return u';
    }
 }.
 
 (* Adversary A3 Against Game3, Constructed from Adversary A2 Against Game2 *)
-module A3(A2 : Adversary) : Adversary = {
-   proc choose(pk : pkey) : plaintext * plaintext = {
-      var pk_dec : seed * Rq_vec;
-      var m0, m1 : plaintext;
+module A3(A2 : Adv_INDCPA_2) : Adv_INDCPA_34 = {
+   proc choose(pk : seed * Rq_vec) : R2 * R2 = {
+      var m0, m1 : R2;
       
       var sd : seed;
       var b : Rq_vec;
       var bp: Rp_vec;
       
-      pk_dec <- pk_decode_g pk;
-      sd <- pk_dec.`1;
-      b <- pk_dec.`2;
+      sd <- pk.`1;
+      b <- pk.`2;
       bp <- Rqv2Rpv b;
       
-      (m0, m1) <@ A2.choose(pk_encode_g (sd, bp));
+      (m0, m1) <@ A2.choose((sd, bp));
       
       return (m0, m1);
    }
 
-   proc guess(c : ciphertext) : bool = {
+   proc guess(c : Rp * Rp_vec) : bool = {
       var u' : bool;
-      var c_dec : Rp * Rp_vec;
       
       var cmu : Rp;
       var b' : Rp_vec;
       var cmu' : Rppq;
       
-      c_dec <- c_decode_g c;
-      cmu <- c_dec.`1;
-      b' <- c_dec.`2;
+      cmu <- c.`1;
+      b' <- c.`2;
       cmu' <- Rp2Rppq cmu; 
       
-      u' <@ A2.guess(c_encode_g (cmu', b'));
+      u' <@ A2.guess((cmu', b'));
 
       return u';
    }
@@ -483,86 +493,86 @@ module A3(A2 : Adversary) : Adversary = {
 
 section Game_Hopping.
 
-(* -- Exclusively Consider Terminating Adversaries -- *)
-declare module A <: Adversary.
-declare axiom Adv_INDCPA_choose_ll : islossless A.choose.
-declare axiom Adv_INDCPA_guess_ll : islossless A.guess.
+(* -- Declare Adversary Against Game0 and Game1  -- *)
+declare module Adv_01 <: Adv_INDCPA.
 
 (* Saber's INDCPA <==> Game 0 *)
 lemma Equivalence_SaberINDCPA_Game0 &m :
-  `| Pr[CPA(Saber_PKE_Scheme, A).main() @ &m : res] - 1%r / 2%r |
+  `| Pr[CPA(Saber_PKE_Scheme, Adv_01).main() @ &m : res] - 1%r / 2%r |
   =
-  `| Pr[Game0(A).main() @ &m : res] - 1%r /2%r |.
+  `| Pr[Game0(Adv_01).main() @ &m : res] - 1%r /2%r |.
 proof.
-have -> //: Pr[CPA(Saber_PKE_Scheme, A).main() @ &m : res] = Pr[Game0(A).main() @ &m : res].
+have -> //: Pr[CPA(Saber_PKE_Scheme, Adv_01).main() @ &m : res] 
+            = 
+            Pr[Game0(Adv_01).main() @ &m : res].
 + byequiv => //.
   proc; inline *. 
   swap {1} 7 -6.
-  call (_ : true); auto; call (_: true); auto.
-  progress; first by rewrite eq_pks_pkg_enc.
-  - by rewrite eq_cs_cg_enc pks_enc_dec_inv.
-  - by rewrite (eq_sym result_R0 bL).
+  call (_ : true); auto; call (_: true); auto => /> u _ sd _ s1 _ s2 _ u'.
+  by rewrite (eq_sym u u').
 qed.
 
 (* Step 1: Game0 <> Game1 -- GMLWR *)
 lemma Step_Distinguish_Game0_Game1_GMLWR &m :
-  `| Pr[Game0(A).main() @ &m : res] - Pr[Game1(A).main() @ &m : res] |
+  `| Pr[Game0(Adv_01).main() @ &m : res] - Pr[Game1(Adv_01).main() @ &m : res] |
   = 
-  `| Pr[GMLWR( B0(A) ).main(true) @ &m : res] - Pr[GMLWR( B0(A) ).main(false) @ &m : res] |. 
+  `| Pr[GMLWR( B0(Adv_01) ).main(true) @ &m : res] - Pr[GMLWR( B0(Adv_01) ).main(false) @ &m : res] |. 
 proof.
-have ->: Pr[Game0(A).main() @ &m : res] =  Pr[GMLWR( B0(A) ).main(false) @ &m : res].
+have ->: Pr[Game0(Adv_01).main() @ &m : res] =  Pr[GMLWR( B0(Adv_01) ).main(false) @ &m : res].
 + byequiv => //.
   proc; inline *.
   rcondf {2} 4.
   - by move=> &m0; auto.
   swap {2} 7 -6; wp.
   by call (_ : true); auto; call (_: true); auto.
-have ->: Pr[Game1(A).main() @ &m : res] =  Pr[GMLWR( B0(A) ).main(true) @ &m : res].
+have ->: Pr[Game1(Adv_01).main() @ &m : res] =  Pr[GMLWR( B0(Adv_01) ).main(true) @ &m : res].
 + byequiv => //.
   proc; inline *.
   rcondt {2} 4.
   - by move=> &m0; auto.
   swap {2} 7 -6; wp.
-  call (_ : true); auto; call (_: true); auto; rnd {2}; auto.
-  by progress; apply dsmallRq_vec_ll.
+  call (_ : true); auto; call (_: true); auto; rnd {2}; auto => /> *.
+  by apply dsmallRq_vec_ll.
 by apply distrC.
 qed.
 
 (* Step 2: Game1 -- Game2 *)
 lemma Step_Game1_Game2 &m :
-  `| Pr[Game1(A).main() @ &m : res] - 1%r / 2%r |
+  `| Pr[Game1(Adv_01).main() @ &m : res] - 1%r / 2%r |
   =
-  `| Pr[Game2( A2(A) ).main() @ &m : res] - 1%r / 2%r |.
+  `| Pr[Game2( A2(Adv_01) ).main() @ &m : res] - 1%r / 2%r |.
 proof.
-have -> //: Pr[Game1(A).main() @ &m : res] = Pr[Game2( A2(A) ).main() @ &m : res].
+have -> //: Pr[Game1(Adv_01).main() @ &m : res] = Pr[Game2( A2(Adv_01) ).main() @ &m : res].
 + byequiv => //.
   proc; inline *.
-  wp; call (_ : true); auto; call (_ : true); auto.
-  by progress; do! congr; rewrite cg_enc_dec_inv; 1: rewrite scaleRp2Rppq2R2t_comp.  
+  wp; call (_ : true); auto; call (_ : true); auto => /> u _ sd _ b _ r s _.
+  by rewrite scaleRp2Rppq2R2t_comp.  
 qed.
+
+
+(* Declare Adversary Against Game2  *)
+declare module Adv_2 <: Adv_INDCPA_2.
 
 (* Auxiliary Step (Reduction 2-3): Game2 -- Game2a *)
 lemma AuxStep_Game2_Game2a &m :
-  `| Pr[Game2(A).main() @ &m : res] - 1%r / 2%r |
+  `| Pr[Game2(Adv_2).main() @ &m : res] - 1%r / 2%r |
   =
-  `| Pr[Game2a(A).main() @ &m : res] - 1%r / 2%r |.
+  `| Pr[Game2a(Adv_2).main() @ &m : res] - 1%r / 2%r |.
 proof.
-have -> //: Pr[Game2(A).main() @ &m : res] = Pr[Game2a(A).main() @ &m : res].
+have -> //: Pr[Game2(Adv_2).main() @ &m : res] = Pr[Game2a(Adv_2).main() @ &m : res].
 + byequiv => //.
   proc; inline *.
-  auto; call(_ : true); auto; call(_ : true); auto.
-  progress.
-  - by rewrite dRqv2dRpv.
-  - by rewrite dRqv2dRpv &(is_fullP dRp_vec) dRp_vec_fu.
+  auto; call(_ : true); auto; call(_ : true); auto => />.
+  by rewrite dRqv2dRpv.
 qed.
 
 (* Auxiliary Step (Reduction 2-3): Game2a -- Game2b *)
 lemma AuxStep_Game2a_Game2b &m :
-  `| Pr[Game2a(A).main() @ &m : res] - 1%r / 2%r |
+  `| Pr[Game2a(Adv_2).main() @ &m : res] - 1%r / 2%r |
   =
-  `| Pr[Game2b(A).main() @ &m : res] - 1%r / 2%r |.
+  `| Pr[Game2b(Adv_2).main() @ &m : res] - 1%r / 2%r |.
 proof.
-have -> //: Pr[Game2a(A).main() @ &m : res] = Pr[Game2b(A).main() @ &m : res].
+have -> //: Pr[Game2a(Adv_2).main() @ &m : res] = Pr[Game2b(Adv_2).main() @ &m : res].
 + byequiv => //.
   proc.
   by auto; call(_ : true); auto; call(_ : true); call sample; auto.
@@ -570,37 +580,39 @@ qed.
 
 (* Auxiliary Step (Reduction 2-3): Game2b -- Game3 *)
 lemma AuxStep_Game2b_Game3 &m :
-  `| Pr[Game2b(A).main() @ &m : res] - 1%r / 2%r |
+  `| Pr[Game2b(Adv_2).main() @ &m : res] - 1%r / 2%r |
   =
-  `| Pr[Game3( A3(A) ).main() @ &m : res] - 1%r / 2%r |.
+  `| Pr[Game3( A3(Adv_2) ).main() @ &m : res] - 1%r / 2%r |.
 proof.
-have -> //: Pr[Game2b(A).main() @ &m : res] = Pr[Game3( A3(A) ).main() @ &m : res].
+have -> //: Pr[Game2b(Adv_2).main() @ &m : res] = Pr[Game3( A3(Adv_2) ).main() @ &m : res].
 + byequiv => //.
   proc; inline *.
-  auto; call(_ : true); auto; call(_ : true); auto.
-  progress.
-  - by rewrite pkg_enc_dec_inv.
-  - rewrite cg_enc_dec_inv /=; congr.
-    rewrite &(pw_eq) // eq_comp23; do 2! congr.
-    by rewrite eq_sym &(Rq2Rp_DG23).
+  auto; call(_ : true); auto; call(_ : true); auto => /> u _ sd _ x _ r s _.
+  by rewrite eq_comp23; do 2! congr; rewrite -Rq2Rp_DG23.
 qed.
 
 (* Step 3: Game2 -- Game3 *)
 lemma Step_Game2_Game3 &m :
-  `| Pr[Game2(A).main() @ &m : res] - 1%r / 2%r |
+  `| Pr[Game2(Adv_2).main() @ &m : res] - 1%r / 2%r |
   =
-  `| Pr[Game3( A3(A) ).main() @ &m : res] - 1%r / 2%r |.
+  `| Pr[Game3( A3(Adv_2) ).main() @ &m : res] - 1%r / 2%r |.
 proof.
 by rewrite (AuxStep_Game2_Game2a &m) (AuxStep_Game2a_Game2b &m) (AuxStep_Game2b_Game3 &m).
 qed.
 
+
+(* Declare (Terminating) Adversary Against Game3 and Game4 *)
+declare module Adv_34 <: Adv_INDCPA_34.
+declare axiom Adv_34_choose_ll : islossless Adv_34.choose.
+declare axiom Adv_34_guess_ll : islossless Adv_34.guess.
+
 (* Step 4: Game3 <> Game4 -- XMLWR *)
 lemma Step_Distinguish_Game3_Game4_XMLWR &m :
-  `| Pr[Game3(A).main() @ &m : res] - Pr[Game4(A).main() @ &m : res] |
+  `| Pr[Game3(Adv_34).main() @ &m : res] - Pr[Game4(Adv_34).main() @ &m : res] |
   = 
-  `| Pr[XMLWR( B1(A) ).main(true) @ &m : res] - Pr[XMLWR( B1(A) ).main(false) @ &m : res] |. 
+  `| Pr[XMLWR( B1(Adv_34) ).main(true) @ &m : res] - Pr[XMLWR( B1(Adv_34) ).main(false) @ &m : res] |. 
 proof.
-have ->: Pr[Game3(A).main() @ &m : res] = Pr[XMLWR( B1(A) ).main(false) @ &m : res].
+have ->: Pr[Game3(Adv_34).main() @ &m : res] = Pr[XMLWR( B1(Adv_34) ).main(false) @ &m : res].
 + byequiv => //.
   proc; inline *.
   rcondf {2} 4.
@@ -609,7 +621,7 @@ have ->: Pr[Game3(A).main() @ &m : res] = Pr[XMLWR( B1(A) ).main(false) @ &m : r
   - by move => &m0; auto.
   swap {2} 11 -10; swap {1} 5 3; swap {2} 6 -2; wp.
   by sim.
-have ->: Pr[Game4(A).main() @ &m : res] = Pr[XMLWR( B1(A) ).main(true) @ &m : res].
+have ->: Pr[Game4(Adv_34).main() @ &m : res] = Pr[XMLWR( B1(Adv_34) ).main(true) @ &m : res].
 + byequiv => //.
   proc; inline *.
   rcondt {2} 4.
@@ -624,12 +636,12 @@ qed.
 
 (* Auxiliary_Game Analysis *)
 lemma Aux_Prob_Half &m :
-  Pr[Auxiliary_Game(A).main() @ &m : res]  = 1%r / 2%r. 
+  Pr[Auxiliary_Game(Adv_34).main() @ &m : res]  = 1%r / 2%r. 
 proof.
 byphoare => //.
 proc.
 rnd.
-call Adv_INDCPA_guess_ll; auto; call Adv_INDCPA_choose_ll; auto.
+call Adv_34_guess_ll; auto; call Adv_34_choose_ll; auto.
 by progress; [apply dseed_ll        |
               apply dRq_vec_ll      |
               apply dRp_vec_ll      |
@@ -639,14 +651,14 @@ qed.
 
 (* Game4 <==> Auxiliary_Game *)
 lemma Equal_Prob_Game4_Aux &m :
-  Pr[Game4(A).main() @ &m : res] = Pr[Auxiliary_Game(A).main() @ &m : res].
+  Pr[Game4(Adv_34).main() @ &m : res] = Pr[Auxiliary_Game(Adv_34).main() @ &m : res].
 proof.
 byequiv => //. 
 proc; inline *.
 swap {2} 7 -6.
 call (_ : true); wp.
-rnd (fun (x : Rp) => x + (scaleR22Rp_var (m_decode (if u{1} then m1{1} else m0{1})) (2 * ep - eq - 1)))  
-    (fun (x : Rp) => x - (scaleR22Rp_var (m_decode (if u{1} then m1{1} else m0{1})) (2 * ep - eq - 1))).
+rnd (fun (x : Rp) => x + (scaleR22Rp_var (if u{1} then m1{1} else m0{1}) (2 * ep - eq - 1)))  
+    (fun (x : Rp) => x - (scaleR22Rp_var (if u{1} then m1{1} else m0{1}) (2 * ep - eq - 1))).
 auto; call(_ : true); auto.
 progress; 1, 4: by ring.
 - by apply /rnd_funi /Rp.dpolyXnD1_funi.
@@ -655,17 +667,17 @@ qed.
 
 (* Game4 Analysis *)
 lemma Game4_Prob_Half &m :
-  Pr[Game4(A).main() @ &m : res] = 1%r / 2%r. 
+  Pr[Game4(Adv_34).main() @ &m : res] = 1%r / 2%r. 
 proof. by rewrite (Equal_Prob_Game4_Aux &m) (Aux_Prob_Half &m). qed.
 
 end section Game_Hopping.
 
 section Security_Theorem.
 
-(* -- Exclusively Consider Terminating Adversaries -- *)
-declare module A <: Adversary.
-declare axiom Adv_INDCPA_choose_ll : islossless A.choose.
-declare axiom Adv_INDCPA_guess_ll : islossless A.guess.
+(* -- Declare (Terminating) Adversary Against INDCPA Game For Saber_PKE_Scheme -- *)
+declare module A <: Adv_INDCPA.
+declare axiom A_choose_ll : islossless A.choose.
+declare axiom A_guess_ll : islossless A.guess.
 
 (* Intelligibility Intermediate Result *)
 lemma Difference_Game1_Game4_XMLWR &m :
@@ -673,12 +685,12 @@ lemma Difference_Game1_Game4_XMLWR &m :
   =
   `| Pr[XMLWR( B1(A3(A2(A))) ).main(true) @ &m : res] - Pr[XMLWR( B1(A3(A2(A))) ).main(false) @ &m : res] |.
 proof.
-move: Adv_INDCPA_choose_ll Adv_INDCPA_guess_ll => c_ll g_ll.
+move: A_choose_ll A_guess_ll => c_ll g_ll.
 rewrite (Game4_Prob_Half (A3(A2(A))))
         3: (Step_Game1_Game2 A)
-        5: (Step_Game2_Game3 (A2(A)))
-        7: -(Game4_Prob_Half (A3(A2(A))) _ _ &m)
-        9: &(Step_Distinguish_Game3_Game4_XMLWR (A3(A2(A)))) //;
+        3: (Step_Game2_Game3 (A2(A)))
+        3: -(Game4_Prob_Half (A3(A2(A))) _ _ &m)
+        5: &(Step_Distinguish_Game3_Game4_XMLWR (A3(A2(A)))) //;
           by proc; inline *; wp; call (_ : true); auto.
 qed.
 
@@ -692,8 +704,8 @@ lemma Saber_INDCPA_Security_Theorem &m :
   `| Pr[XMLWR(BX).main(true) @ &m : res] - Pr[XMLWR(BX).main(false) @ &m : res] |. 
 proof.
 exists (B0(A)) (B1(A3(A2(A)))).
-move: Adv_INDCPA_choose_ll Adv_INDCPA_guess_ll => c_ll g_ll.
-rewrite (Equivalence_SaberINDCPA_Game0 A) 3: -(Game4_Prob_Half (A3(A2(A))) _ _ &m) //;
+move: A_choose_ll A_guess_ll => c_ll g_ll.
+rewrite (Equivalence_SaberINDCPA_Game0 A) -(Game4_Prob_Half (A3(A2(A))) _ _ &m) //;
           first 2 by proc; inline *; wp; call (_ : true); auto.
 have:
   `| Pr[Game0(A).main() @ &m : res] - Pr[Game1(A).main() @ &m : res] |
